# 二项式反演

$$
f(n)=\sum_{i=0}^n\begin{pmatrix}n\\i\end{pmatrix}g(i)\Leftrightarrow g(n)=\sum_{i=0}^n(-1)^{n-i}\begin{pmatrix}n\\i\end{pmatrix}f(i)
$$

### 证明

将$g(n)$带入$f(n)$表达式
$$
\begin{aligned}
f(n)&=\sum_{i=0}^n\begin{pmatrix}n\\i\end{pmatrix}\sum_{j=0}^i(-1)^{i-j}\begin{pmatrix}i\\j\end{pmatrix}f(j)\\
&=\sum_{j=0}^n\sum_{i=j}^n\begin{pmatrix}n\\i\end{pmatrix}(-1)^{i-j}\begin{pmatrix}i\\j\end{pmatrix}f(j)\\
&=\sum_{j=0}^n\begin{pmatrix}n\\j\end{pmatrix}f(j)\sum_{i=j}^n\begin{pmatrix}n-j\\i-j\end{pmatrix}(-1)^{i-j}\\
&=\sum_{j=0}^n\begin{pmatrix}n\\j\end{pmatrix}f(j)(1-1)^{n-j}\\
&=f(n)
\end{aligned}
$$

### 应用

在计数题中，可以将$f(n)$看做最多为$n$个，$g(n)$看做一定为$n$个，二项式反演建立了这两者的关系